Merge some lemmas for L2NL translation.

src/LustreToNLustre/LustreToNLustre.v
@@ -104,16 +104,6 @@ Module Type LUSTRE_TO_NLUSTRE
     | (x, b) :: sfx' => clock_of_suffix sfx' (Con ck x b)
     end.
 
-  (* TODO: move to common *)
-  Lemma app_tail_eq:
-    forall {A} (xs ys zs : list A),
-      xs = zs ->
-      xs ++ ys = zs ++ ys.
-  Proof.
-    intros * Heq. induction ys.
-    now setoid_rewrite app_nil_r.
-    now subst xs.
-  Qed.
 
   Lemma suffix_of_clock_app:
     forall sfx sfx' ck,
@@ -123,8 +113,7 @@ Module Type LUSTRE_TO_NLUSTRE
     induction sfx' as [|xb sfx' IH].
     now setoid_rewrite app_nil_r.
     intros sfx ck.
-    rewrite <-app_last_app, IH, <-app_last_app  with (xs':=sfx').
-    apply app_tail_eq.
+    rewrite <-app_last_app, IH, <-app_last_app  with (xs':=sfx'). f_equal.
     revert sfx; clear.
     induction ck; auto.
     simpl; intros sfx.
@@ -187,8 +176,8 @@ Module Type LUSTRE_TO_NLUSTRE
     | _ => Error (msg "not a constant")
     end.
 
-  Definition to_equation (env : Env.t (type * clock)) (eq : L.equation)
-                                                          : res NL.equation :=
+  Definition to_equation (env : Env.t (type * clock)) (envo : ident -> res unit)
+                         (eq : L.equation) : res NL.equation :=
     match eq with
     | (xs, [L.Eapp f es _]) =>
         do xcks1 <- mmap (find_clock env) xs;
@@ -197,6 +186,7 @@ Module Type LUSTRE_TO_NLUSTRE
         OK (NL.EqApp xs (find_base_clock (xcks1 ++ xcks2)) f les None)
 
     | ([x], [L.Efby [e0] [e] _]) =>
+        do _  <- envo x;
         do c0 <- to_constant e0;
         do ck <- find_clock env x;
         do le <- to_lexp e;
@@ -210,48 +200,728 @@ Module Type LUSTRE_TO_NLUSTRE
     | _ => Error (msg "equation not normalized")
     end.
 
-  Program Definition to_node (n : L.node) : res NL.node :=
-    let env := Env.adds' n.(L.n_out)
-                             (Env.adds' n.(L.n_vars)
-                                            (Env.from_list n.(L.n_in)))
-    in
-    do neqs  <- mmap (to_equation env) n.(L.n_eqs);
-    OK {|
-        NL.n_name     := n.(L.n_name);
-        NL.n_in       := n.(L.n_in);
-        NL.n_out      := n.(L.n_out);
-        NL.n_vars     := n.(L.n_vars);
-        NL.n_eqs      := neqs;
 
-        NL.n_ingt0    := _;
-        NL.n_outgt0   := _;
-        NL.n_defd     := _;
-        NL.n_nodup    := _;
-        NL.n_good     := _
-      |}.
-  Next Obligation.
-    exact (L.n_ingt0 n).
+  Lemma ok_fst_defined eq eq' :
+    forall env envo,
+      to_equation env envo eq = OK eq' -> fst eq = NL.var_defined eq'.
+  Proof.
+    intros env envo Htoeq.
+    unfold to_equation in Htoeq.
+    cases; monadInv Htoeq; inv EQ; simpl; auto.
   Qed.
-  Next Obligation.
-    exact (L.n_outgt0 n).
+
+  Lemma nl_vars_defined_cons:
+    forall eq eqs,
+      NL.vars_defined (eq::eqs) = NL.var_defined eq ++ NL.vars_defined eqs.
+  Proof.
+    intros. unfold NL.vars_defined. now simpl.
   Qed.
-  Next Obligation.
-    admit (* L.vars_defined = NL.vars_defined *).
-  Admitted.
-  Next Obligation.
-    admit.
-  Admitted.
-  Next Obligation.
-    exact (L.n_nodup n).
+
+  Remark mmap_cons:
+    forall (A B: Type) (f: A -> res B) (l: list A) (r: list B) (x: A),
+      mmap f (x :: l) = OK r ->
+      exists x' l', r = x' :: l' /\ f x = OK x' /\ mmap f l = OK l'.
+  Proof.
+    induction l; simpl; intros.
+    monadInv H. exists x0, []. auto.
+    monadInv H. exists x0, x1. auto.
   Qed.
-  Next Obligation.
-    admit.
-  Admitted.
+
+  Remark mmap_cons2:
+    forall (A B: Type) (f: A -> res B) (l: list A) (r: list B) (x: B),
+      mmap f (l) = OK (x :: r) ->
+      exists x' l', l = x' :: l' /\ f x' = OK x /\ mmap f l' = OK r.
+  Proof.
+    induction l; simpl; intros.
+    monadInv H.
+    monadInv H. exists a, l. auto.
+  Qed.
+
+  Definition mmap_to_equation env envo n :
+    res { neqs | mmap (to_equation env envo) n.(L.n_eqs) = OK neqs }.
+  Proof.
+    destruct (mmap (to_equation env envo) n.(L.n_eqs)).
+    left. eauto.
+    right. auto.
+  Defined.
+
+  Definition to_node (n : L.node) : res NL.node.
+    refine (
+        let envo := Env.from_list n.(L.n_out) in
+        let env := Env.adds' n.(L.n_vars) (Env.adds' n.(L.n_in) envo) in
+        let is_not_out :=
+            fun x => if Env.mem x envo
+                  then Error (msg "output variable defined as a fby")
+                  else OK tt in
+        match mmap_to_equation env is_not_out n with
+        | OK (exist neqs P) =>
+          OK {|
+              NL.n_name     := n.(L.n_name);
+              NL.n_in       := n.(L.n_in);
+              NL.n_out      := n.(L.n_out);
+              NL.n_vars     := n.(L.n_vars);
+              NL.n_eqs      := neqs;
+
+              NL.n_ingt0    := L.n_ingt0 n;
+              NL.n_outgt0   := L.n_outgt0 n;
+              NL.n_defd     := _;
+              NL.n_vout     := _;
+              NL.n_nodup    := L.n_nodup n;
+              NL.n_good     := _
+            |}
+        | Error e => Error e
+        end).
+
+  (* NL.n_defd obligation *)
+  {
+    assert (NL.vars_defined neqs = L.vars_defined (L.n_eqs n)).
+    { revert neqs P. induction (L.n_eqs n); simpl.
+    - intros neqs Htr. inv Htr. auto.
+    - intros neqs Htoeq. monadInv Htoeq.
+      apply IHl in EQ1. simpl.
+      apply ok_fst_defined in EQ. rewrite EQ1. now rewrite <- EQ.
+      eauto.
+    }
+    rewrite H.
+    exact (L.n_defd n).
+  }
+
+  (* NL.n_vout obligation *)
+  {
+    intros xo Hin.
+    monadInv P. induction H as [| eq leq eq' leq' Htoeq ].
+    intro Hbad. inv Hbad.
+    assert (Hmmap := P).
+    apply mmap_cons2 in P.
+    destruct P as (eq'' & leq'' & Heqs' & Htoeq' & Hmmap').
+    inv Heqs'.
+    simpl. destruct (NL.is_fby eq') eqn:?.
+    - unfold NL.vars_defined, flat_map. simpl. rewrite in_app.
+      intro Hi. destruct Hi.
+      + unfold to_equation in Htoeq. destruct eq''.
+        cases; monadInv Htoeq; inv Heqb. simpl in H0. destruct H0; auto. subst.
+        unfold is_not_out in EQ. cases_eqn EQ. inv EQ.
+        apply Env.Props.P.F.not_mem_in_iff in EQ3. unfold envo in EQ3.
+        apply EQ3.
+        rewrite in_map_iff in Hin.
+        destruct Hin as ((x & ?) & Hfst & Hin). inv Hfst.
+        eapply Env.find_In. eapply Env.In_find_adds'; simpl; eauto.
+        destruct n. simpl. assert (Hnodup := n_nodup).
+        now repeat apply NoDupMembers_app_r in Hnodup.
+      + apply IHlist_forall2; auto. exists leq'; auto.
+    - apply IHlist_forall2. exists leq'; auto. assumption.
+  }
+
+  (* NL.n_good obligation *)
+  {
+    Axiom AXIOM_VALID_TODO_REMOVE_ME :
+      forall id, valid id.
+    repeat split.
+    - apply Forall_Forall. exact n.(L.n_good).
+      (* TODO: valid in, vars, vars *)
+      apply Forall_forall; intros; apply AXIOM_VALID_TODO_REMOVE_ME.
+    - (* TODO: valid n_name *)
+      apply AXIOM_VALID_TODO_REMOVE_ME.
+  }
+
+  Defined. (* to_node *)
 
   Definition to_global (g : L.global) : res NL.global :=
     mmap to_node g.
 
-  (* TODO: Show semantic preservation. *)
+
+
+  (* Proofs for semantics *)
+
+  Ltac tonodeInv H :=
+    match type of H with
+    | (to_node ?n = OK _) =>
+      let Hs := fresh in
+      let Hmmap := fresh "Hmmap" in
+      unfold to_node in H;
+      destruct(mmap_to_equation
+               (Env.adds' (L.n_vars n)
+                (Env.adds' (L.n_in n)
+                 (Env.from_list (L.n_out n))))
+            (fun x : Env.key =>
+             if Env.mem x (Env.from_list (L.n_out n))
+             then Error (msg "output variable defined as a fby")
+             else OK tt) n)
+      as [ Hs | Hs ];
+      try (destruct Hs as (? & Hmmap)); inv H
+    end.
+
+  Lemma find_node_hd f a G n :
+    L.find_node f (a :: G) = Some n ->
+    ((ident_eqb (L.n_name a) f) = true  /\ a = n) \/
+    ((ident_eqb (L.n_name a) f) = false /\ L.find_node f G = Some n).
+  Proof.
+    simpl. intro.
+    case_eq (ident_eqb (L.n_name a) f); intro; rewrite H0 in H; inv H.
+    auto. right. auto.
+  Qed.
+
+  Lemma find_node_In :
+    forall f G n, L.find_node f G = Some n -> In n G.
+  Proof.
+    induction G; intros * Hfind; try discriminate.
+    inv Hfind. destruct (ident_eqb (L.n_name a) f).
+    inv H0. simpl. now left.
+    simpl. right. now apply IHG.
+  Qed.
+
+  Lemma to_node_name n n' :
+    to_node n = OK n' -> L.n_name n = NL.n_name n'.
+  Proof.
+    (* intro Htr. tonodeInv Htr. auto. *)
+    (* Qed. *)
+  Admitted.
+
+  Lemma to_node_in n n' :
+    to_node n = OK n' -> (LS.idents (L.n_in n)) = (NLSC.idents (NL.n_in n')).
+  Proof.
+    (* intro Htr. tonodeInv Htr. auto. *)
+    (* Qed. *)
+  Admitted.
+
+  Lemma to_node_out n n' :
+    to_node n = OK n' -> (LS.idents (L.n_out n)) = (NLSC.idents (NL.n_out n')).
+  Proof.
+    (* intro Htr. tonodeInv Htr. auto. *)
+    (* Qed. *)
+  Admitted.
+
+
+  Lemma find_node_global (G: L.global) (P: NL.global) (f: ident) (n: L.node) :
+    to_global G = OK P ->
+    L.find_node f G = Some n ->
+    exists n', NL.find_node f P = Some n' /\ to_node n = OK n'.
+  Proof.
+    revert P.
+    induction G; intros P Htrans Hfind. inversion Hfind.
+    apply find_node_hd in Hfind.
+    destruct Hfind.
+    - inv H. apply mmap_cons in Htrans.
+      destruct Htrans as [ n' [ l' [ Hp [ Hnode Hmmap ]]]]; subst.
+      exists n'.
+      remember Hnode as Heq; clear HeqHeq. apply to_node_name in Heq.
+      split; auto. simpl. rewrite <- Heq. rewrite H0. reflexivity.
+    - destruct H as [ Hneq Hfind ].
+      apply mmap_cons in Htrans.
+      destruct Htrans as [ n' [P' [nP [Hton  Htrans]]]]. subst.
+      apply IHG in Htrans; auto. destruct Htrans. destruct H as [ H Hnode ].
+      exists x. split; auto. apply NL.find_node_other; auto.
+      apply to_node_name in Hton. rewrite <- Hton. apply ident_eqb_neq. auto.
+  Qed.
+
+  Lemma const_eq :
+    forall c b, NLSC.const c b ≡ LS.const c b.
+  Proof.
+    cofix Cofix. intros.
+    unfold_Stv b; constructor; simpl; auto.
+  Qed.
+
+  Lemma const_inv1 :
+    forall c b s,
+      LS.const c b ≡ absent ::: s ->
+      exists b', s ≡ LS.const c b' /\ b ≡ false ::: b'.
+  Proof.
+    intros * H.
+    unfold_Stv b; inv H; simpl in *; inv H0.
+    exists b. split; symmetry; auto. reflexivity.
+  Qed.
+
+  Lemma const_inv2 :
+    forall c c' b s,
+      LS.const c b ≡ present c' ::: s ->
+      exists b', s ≡ LS.const c b'
+            /\ b ≡ true ::: b'
+            /\ c' = sem_const c.
+  Proof.
+    intros * H.
+    unfold_Stv b; inv H; simpl in *; inv H0.
+    exists b. split. symmetry. assumption. split; reflexivity.
+  Qed.
+
+  Lemma const_tl :
+    forall c b v tl,
+      LS.const c b ≡ v ::: tl ->
+      LS.const c (Streams.tl b) ≡ tl.
+  Proof.
+    intros * H.
+    unfold_Stv b; inv H; simpl in *; inv H0; assumption.
+  Qed.
+
+  Lemma sem_var_var :
+    forall H x s,
+      LS.sem_var H x s <-> NLSC.sem_var H x s.
+  Proof.
+    split; intros * Hsem; inv Hsem;
+    econstructor; eauto.
+  Qed.
+
+  Lemma env_maps_tl :
+    forall i v s H,
+      Env.MapsTo i (v ::: s) H -> Env.MapsTo i s (NLSC.History_tl H).
+  Proof.
+    intros * Hmap.
+    unfold NLSC.History_tl.
+    assert (s = Streams.tl (v ::: s)) as Hs by auto.
+    rewrite Hs. eapply Env.map_1. assumption.
+  Qed.
+
+  Lemma sem_var_step :
+    forall H x v s,
+      LS.sem_var H x (v ::: s) -> LS.sem_var (NLSC.History_tl H) x s.
+  Proof.
+    intros * Hsem.
+    inv Hsem.
+    destruct xs'.
+    econstructor.
+    eapply env_maps_tl; eauto. now inv H2.
+  Qed.
+
+  Lemma sem_clock_step :
+    forall H b ck s ss,
+      NLSC.sem_clock H b ck (s ::: ss) ->
+      NLSC.sem_clock (NLSC.History_tl H) (Streams.tl b) ck ss.
+  Proof.
+    intros * Hsem.
+    inv Hsem; auto. econstructor. rewrite H1. simpl. reflexivity.
+  Qed.
+
+  Lemma sem_const_step :
+    forall G H b e e' v s,
+      to_constant e = OK e' ->
+      LS.sem_exp G H b e [v ::: s] ->
+      LS.sem_exp G (NLSC.History_tl H) (Streams.tl b) e [s].
+  Proof.
+    einduction e using L.exp_ind2; intros * Htr Hsem; inv Htr.
+    - inv Hsem. symmetry in H5.
+      destruct v;
+        [ apply const_inv1 in H5; destruct H5 as [ b' [ Hs Hb ] ]
+        | apply const_inv2 in H5; destruct H5 as (b' & Hs & Hb & Hc) ];
+        rewrite Hs; rewrite Hb; simpl; econstructor; reflexivity.
+    - destruct es; inv H2.
+      destruct es; inv H3.
+      inv H0. inv H5. inv Hsem. inv H12. inv H10. inv H9. inv H6. inv H0.
+      rewrite app_nil_r in H3. inv H3.
+      destruct x0. destruct s0.
+      econstructor. econstructor; eauto.
+      eapply sem_var_step; eauto. econstructor; eauto.
+      now inv H5.
+  Qed.
+
+    Lemma sem_lexp_step :
+    forall G H b e e' v s,
+      to_lexp e = OK e' ->
+      LS.sem_exp G H b e [v ::: s] ->
+      LS.sem_exp G (NLSC.History_tl H) (Streams.tl b) e [s].
+  Proof.
+    einduction e using L.exp_ind2; intros * Htr Hsem; inv Htr.
+    - inv Hsem. symmetry in H5.
+      destruct v;
+        [ apply const_inv1 in H5; destruct H5 as [ b' [ Hs Hb ] ]
+        | apply const_inv2 in H5; destruct H5 as (b' & Hs & Hb & Hc) ];
+      rewrite Hs; rewrite Hb; simpl; econstructor; reflexivity.
+    - inv Hsem. inv H5.  destruct xs'.
+      econstructor. econstructor.
+      eapply env_maps_tl; eauto. inv H3; simpl in *. assumption.
+    - inv Hsem. destruct a. monadInv H1. destruct s0.
+      econstructor; eauto. inv H10; auto.
+    - inv Hsem. destruct a. monadInv H1. destruct s1, s2.
+      econstructor; eauto. inv H13; auto.
+    - destruct es; inv H2.
+      destruct es; inv H3.
+      inv H0.
+      destruct a. destruct l; inv H2.
+      destruct l; try now inv H1. monadInv H1.
+      clear H5.
+      inv Hsem. inv H11. inv H5. destruct s0, x1.
+      inv H9. inv H7. simpl in H0. rewrite app_nil_r in H0. subst.
+      econstructor.
+      + econstructor; eauto.
+      + eapply sem_var_step. eassumption.
+      + econstructor; eauto. inv H3; eauto.
+  Qed.
+
+  Lemma sem_cexp_step :
+    forall G H b e e' v s,
+      to_cexp e = OK e' ->
+      LS.sem_exp G H b e [v ::: s] ->
+      LS.sem_exp G (NLSC.History_tl H) (Streams.tl b) e [s].
+  Proof.
+    einduction e using L.exp_ind2; intros * Htr Hsem;
+      (now inv Htr) || (unfold to_cexp in Htr;
+                       try (monadInv Htr; eapply sem_lexp_step; eauto));
+      cases; monadInv Htr; fold to_cexp in *;
+
+        inv Hsem; inv H11; inv H6; inv H12; inv H7; inv H13; inv H10;
+          rewrite app_nil_r in H3, H2; subst;
+            inv H0; inv H1; clear H10 H7; destruct x2, y1.
+    - inv H8;
+        (econstructor; eauto;
+         [ eapply sem_var_step; eauto | econstructor; eauto; econstructor ]).
+    - inv H8;
+        (econstructor; eauto; eapply sem_lexp_step in EQ; eauto;
+         econstructor; eauto; constructor).
+  Qed.
+
+  Lemma lift1_id :
+    forall op ty xs rs, LS.lift1 op ty xs rs -> NLSC.lift1 op ty xs rs.
+  Proof.
+    cofix Cofix.
+    intros * Hlift.
+    unfold_Stv xs; unfold_Stv rs; inv Hlift;
+      econstructor; eauto; eapply Cofix; eauto.
+  Qed.
+
+  Lemma lift2_id :
+    forall op ty1 ty2 xs ys rs,
+      LS.lift2 op ty1 ty2 xs ys rs -> NLSC.lift2 op ty1 ty2 xs ys rs.
+  Proof.
+    cofix Cofix.
+    intros * Hlift.
+    unfold_Stv xs; unfold_Stv rs; inv Hlift;
+      econstructor; eauto; eapply Cofix; eauto.
+  Qed.
+
+  Lemma when_id :
+    forall k xs cs rs, LS.when k cs xs rs -> NLSC.when k xs cs rs.
+  Proof.
+    cofix Cofix.
+    intros * Hwhen.
+    unfold_Stv xs; unfold_Stv cs; inv Hwhen;
+      econstructor; eauto; eapply Cofix; eauto.
+  Qed.
+
+  Lemma merge_id :
+    forall k xs cs rs, LS.merge k xs cs rs -> NLSC.merge k xs cs rs.
+  Proof.
+    cofix Cofix.
+    intros * Hwhen.
+    unfold_Stv xs; unfold_Stv cs; inv Hwhen;
+      econstructor; eauto; eapply Cofix; eauto.
+  Qed.
+
+  Lemma ite_id :
+    forall k xs cs rs, LS.ite k xs cs rs -> NLSC.ite k xs cs rs.
+  Proof.
+    cofix Cofix.
+    intros * Hwhen.
+    unfold_Stv xs; unfold_Stv cs; inv Hwhen;
+      econstructor; eauto; eapply Cofix; eauto.
+  Qed.
+
+  Lemma ty_lexp :
+    forall G env e e',
+      LT.wt_exp G env e ->
+      to_lexp e = OK e' ->
+      L.typeof e = [CE.typeof e'].
+  Proof.
+    induction e using L.exp_ind2; intros * Hwt Htr; inv Htr.
+    - now simpl.
+    - destruct a. inv H0. now simpl.
+    - destruct a. simpl. monadInv H0. now simpl.
+    - destruct a. monadInv H0. now simpl.
+    - cases. inv H. simpl. inv Hwt. inv H8. inv H6. monadInv H1.
+      unfold L.typesof. unfold flat_map. simpl. rewrite app_nil_r.
+      now apply H3.
+  Qed.
+
+  Lemma sem_lexp_single :
+    forall e e' G H b ss,
+      to_lexp e = OK e' ->
+      LS.sem_exp G H b e ss ->
+      exists s, ss = [s].
+  Proof.
+    induction e using L.exp_ind2; intros * Htr Hsem; inv Htr;
+      try (inv Hsem; eexists; now eauto).
+    cases_eqn H2. subst. monadInv H2. inv Hsem. inv H9. inv H5. inv H. inv H5.
+    eapply H4 in EQ; [|eauto]. inv EQ. simpl in H11. inv H11. inv H6.
+    eauto.
+  Qed.
+
+  Lemma sem_exp_lexp :
+    forall G G' env H b e e' s,
+      LT.wt_exp G' env e ->
+      to_lexp e = OK e' ->
+      LS.sem_exp G H b e [s] ->
+      NLSC.sem_lexp H b e' s.
+  Proof.
+    induction e using L.exp_ind2; intros * Hwt Htr Hsem; inv Htr.
+    - inv Hsem. econstructor. now rewrite const_eq.
+    - destruct a. inv Hsem. inv H1. econstructor. now apply sem_var_var.
+    - destruct a. inv Hsem. monadInv H1. inv Hwt. econstructor; eauto.
+      apply lift1_id. eapply ty_lexp in EQ; eauto. rewrite H9 in EQ. now inv EQ.
+    - destruct a. inv Hsem. monadInv H1. inv Hwt. econstructor; eauto.
+      apply lift2_id. eapply ty_lexp in EQ; eauto. eapply ty_lexp in EQ1; eauto.
+      rewrite H11 in EQ. inv EQ. rewrite H12 in EQ1. now inv EQ1.
+    - cases. monadInv H2. inv Hsem. inv H0. clear H4. inv Hwt.
+      inv H9. inv H5. inv H11. inv H6. rewrite app_nil_r in H0. inv H0. inv H14.
+      econstructor. eapply H3; eauto. eapply sem_var_var. eassumption.
+      now eapply when_id.
+  Qed.
+
+  Lemma sem_exp_cexp :
+    forall G G' env H b e e' s,
+      LT.wt_exp G' env e ->
+      to_cexp e = OK e' ->
+      LS.sem_exp G H b e [s] ->
+      NLSC.sem_cexp H b e' s.
+  Proof.
+    induction e using L.exp_ind2; intros * Hwt Htr Hsem;
+      (now inv Htr) || (unfold to_cexp in Htr;
+                       try (monadInv Htr; econstructor;
+                            eapply sem_exp_lexp; eauto));
+      cases; monadInv Htr; fold to_cexp in *;
+                 inv Hsem; inv H11; inv H6; inv H12; inv H7; inv H13; inv H10;
+                   rewrite app_nil_r in H3, H2; subst;
+                     inv H0; inv H1; clear H10 H7; destruct x2, y1.
+    - inv Hwt; inv H11; inv H12. inv H8;
+        (econstructor; eauto;
+         [ eapply sem_var_var; eauto
+         | econstructor; eauto; eapply merge_id; eauto ]).
+    - inv Hwt. inv H12. inv H13.
+      inv H8; econstructor; eauto;
+        eapply sem_exp_lexp in EQ; eauto;
+          econstructor; now apply ite_id.
+  Qed.
+
+  CoFixpoint abstract_clock (xs: Stream value) : Stream bool:=
+    match xs with
+    | absent ::: xs => false ::: abstract_clock xs
+    | present _ ::: xs => true ::: abstract_clock xs
+    end.
+
+  Lemma length_typeof :
+    forall G H b env e os,
+      LT.wt_exp G env e ->
+      LS.sem_exp G H b e os ->
+      length (L.typeof e) = length os.
+  Proof.
+    induction e using L.exp_ind2; intros * Hwt Hsem;
+      try (inv Hsem; inv Hwt; simpl; reflexivity).
+    - inv Hsem. inv Hwt. simpl.
+      rewrite <- H7. apply Forall3_length in H11. destruct H11.
+      rewrite <- H3. unfold L.typesof, flat_map.
+      clear H7 H9 H2 H3. revert dependent sss. induction es; intros.
+      + inv H10. auto.
+      + inv H10. inv H1. inv H6. simpl.
+        rewrite app_length. rewrite app_length.
+        f_equal. apply H7; auto.
+        apply IHes; auto.
+    - inv Hsem. inv Hwt. simpl.
+      apply Forall2_length in H11. rewrite <- H11.
+      clear H11. revert dependent ss. induction es; intros.
+      + inv H9. auto.
+      + inv H9. inv H0. inv H5. unfold L.typesof, flat_map. simpl.
+        rewrite app_length. rewrite app_length.
+        f_equal. apply H4; auto.
+        apply IHes; auto.
+    - inv Hsem. inv Hwt. simpl.
+      apply Forall3_length in H13. destruct H13.
+      rewrite <- H3, <- H2. unfold L.typesof, flat_map.
+      clear H7 H9 H2 H3 H14. revert dependent ts. induction ets; intros.
+      + inv H11. auto.
+      + inv H11. inv H0. inv H6. simpl.
+        rewrite app_length. rewrite app_length.
+        f_equal. apply H5; auto.
+        apply IHets; auto.
+    - inv Hsem. inv Hwt. simpl.
+      apply Forall3_length in H13. destruct H13.
+      rewrite <- H3, <- H2. unfold L.typesof, flat_map.
+      clear H9 H2 H3 H15. revert dependent ts. induction ets; intros.
+      + inv H11. auto.
+      + inv H11. inv H0. inv H7. simpl.
+        rewrite app_length. rewrite app_length.
+        f_equal. apply H5; auto.
+        apply IHets; auto.
+    - inv Hsem. inv H9. inv Hwt. rewrite H2 in H12. inv H12.
+      simpl. rewrite map_length.
+      apply Forall2_length in H14. rewrite H14.
+      apply Forall2_length in H4. rewrite <- H4.
+      clear - n0.
+      induction (L.n_out n0); auto. simpl. f_equal. apply IHl.
+  Qed.
+
+  Lemma length_clockof :
+    forall G H b env e os,
+      LC.wc_exp G env e ->
+      LS.sem_exp G H b e os ->
+      length (L.clockof e) = length os.
+  Proof.
+    induction e using L.exp_ind2; intros * Hwc Hsem;
+      try (inv Hsem; inv Hwc; simpl; reflexivity); inv Hsem.
+    - inv Hwc. simpl.
+      apply Forall2_length in H7. rewrite H7.
+      apply Forall3_length in H11. destruct H11.
+      rewrite <- H3, <- H2. unfold L.clocksof, flat_map.
+      clear H2 H3 H7.
+      revert dependent s0ss. induction e0s; intros.
+      + inv H8. auto.
+      + inv H8. inv H0. simpl.
+        rewrite app_length. rewrite app_length. inv H5.
+        f_equal. apply H7; auto.
+        apply IHe0s; auto.
+    - inv Hwc. simpl. rewrite map_length. rewrite H8.
+      apply Forall2_length in H11. rewrite <- H11.
+      clear H11 H7 H8. revert dependent ss. induction es; intros.
+      + inv H9. auto.
+      + inv H9. inv H0. inv H5. unfold L.clocksof, flat_map. simpl.
+        rewrite app_length. rewrite app_length.
+        f_equal. apply H4; auto.
+        apply IHes; auto.
+    - inv Hwc. simpl. rewrite map_length. rewrite H15.
+      apply Forall3_length in H13. destruct H13.
+      rewrite <- H3, <- H2. unfold L.clocksof, flat_map.
+      clear H7 H9 H2 H3 H14 H10 H15 H16. revert dependent ts.
+      induction ets; intros.
+      + inv H11. auto.
+      + inv H11. inv H0. inv H6. simpl.
+        rewrite app_length. rewrite app_length.
+        f_equal. apply H5; auto.
+        apply IHets; auto.
+    - inv Hwc. simpl. rewrite map_length. rewrite H16.
+      apply Forall3_length in H13. destruct H13.
+      rewrite <- H3, <- H2. unfold L.clocksof, flat_map.
+      clear H9 H2 H3 H15 H14 H16 H17. revert dependent ts.
+      induction ets; intros.
+      + inv H11. auto.
+      + inv H11. inv H0. inv H7. simpl.
+        rewrite app_length. rewrite app_length.
+        f_equal. apply H5; auto.
+        apply IHets; auto.
+    - inv H9. inv Hwc. rewrite H2 in H12. inv H12.
+      apply Forall2_length in H4. rewrite <- H4.
+      destruct H13 as (?&?&?&Hnout).
+      apply Forall2_length in Hnout. rewrite map_length in Hnout.
+      simpl. rewrite map_length. rewrite <- Hnout.
+      clear - n0.
+      induction (L.n_out n0); auto. simpl. f_equal. apply IHl.
+  Qed.
+
+  Lemma ac_when :
+    forall k cs xs rs,
+      LS.when k cs xs rs -> abstract_clock cs ≡ abstract_clock xs.
+  Proof.
+    cofix Cofix.
+    intros * Hwhen. inv Hwhen; econstructor; simpl; eauto.
+  Qed.
+
+  Lemma ac_const:
+    forall c b cs,
+      LS.const c b ≡ cs -> b ≡ abstract_clock cs.
+  Proof.
+    cofix Cofix.
+    intros * Hconst.
+    unfold_Stv b;
+      inv Hconst; simpl in *;
+      unfold_Stv cs; constructor; simpl; eauto; inv H.
+  Qed.
+
+  Lemma ac_fby :
+    forall xs ys rs,
+      LS.fby xs ys rs -> abstract_clock xs ≡ abstract_clock rs.
+  Proof.
+    cofix Cofix.
+    intros * Hfby.
+    unfold_Stv xs; inv Hfby; econstructor; simpl; eauto.
+    clear - H3. revert H3. revert y xs ys0 rs0.
+    cofix Cofix.
+    intros * Hfby1.
+    unfold_Stv xs; inv Hfby1; econstructor; simpl; eauto.
+  Qed.
+
+  Lemma ac_ite :
+    forall s  ts fs rs,
+      LS.ite s ts fs rs -> abstract_clock ts ≡ abstract_clock rs.
+  Proof.
+    cofix Cofix.
+    intros * Hite.
+    unfold_Stv ts; inv Hite; econstructor; simpl; eauto.
+  Qed.
+
+  Lemma ac_lift1 :
+    forall op ty s o,
+      LS.lift1 op ty s o -> abstract_clock s ≡ abstract_clock o.
+  Proof.
+    cofix Cofix.
+    intros * Hlift.
+    unfold_Stv s; inv Hlift; econstructor; simpl; eauto.
+  Qed.
+
+  Lemma ac_lift2 :
+    forall op ty1 ty2 s1 s2 o,
+      LS.lift2 op ty1 ty2 s1 s2 o -> abstract_clock s1 ≡ abstract_clock o.
+  Proof.
+    cofix Cofix.
+    intros * Hlift.
+    unfold_Stv s1; inv Hlift; econstructor; simpl; eauto.
+  Qed.
+
+  Inductive Is_free_left (x : ident) : L.exp -> Prop :=
+  | IFLvar : forall a,
+      Is_free_left x (L.Evar x a)
+  | IFLunop : forall op e a,
+      Is_free_left x e ->
+      Is_free_left x (L.Eunop op e a)
+  | IFLbinop : forall op e1 e2 a,
+      Is_free_left x e1
+      \/ Is_free_left x e2 ->
+      Is_free_left x (L.Ebinop op e1 e2 a)
+  | IFLfby : forall e0s es a,
+      Exists (Is_free_left x) e0s ->
+      Is_free_left x (L.Efby e0s es a)
+  | IFLwhen : forall es y b a,
+      x = y
+      \/ Exists (Is_free_left x) es ->
+      Is_free_left x (L.Ewhen es y b a)
+  | IFLmerge : forall ets efs y a,
+      x = y
+      \/ Exists (Is_free_left x) ets
+      \/ Exists (Is_free_left x) efs ->
+      Is_free_left x (L.Emerge y ets efs a)
+  | IFLite : forall e ets efs a,
+      Is_free_left x e
+      \/ Exists (Is_free_left x) ets
+      \/ Exists (Is_free_left x) efs ->
+      Is_free_left x (L.Eite e ets efs a)
+  | IFLapp : forall f es a,
+      Exists (Is_free_left x) es ->
+      Is_free_left x (L.Eapp f es a).
+
+  Lemma Forall2_const_map :
+    forall (A B C : Type) (P : A -> B -> Prop) (e : A) (l : list C) (l' : list B),
+      Forall (fun y => P e y) l' ->
+      length l = length l' ->
+      Forall2 (fun x y => P x y) (map (fun _ => e) l) l'.
+  Proof.
+    intros * Hf Hlen.
+    apply Forall2_forall; split; [| now rewrite map_length].
+    intros * Hin. revert dependent l'.
+    induction l; intros. inv Hin.
+    destruct l'; inv Hlen. simpl in Hin.
+    destruct Hin; inv Hf; try inv H; eauto.
+  Qed.
+
+  Definition var_inv (D : positive -> Prop) (env : list (ident * clock)) : Prop :=
+    forall x, D x ->
+         (forall H b ck x xs,
+             In (x, ck) env ->
+             LS.sem_var H x xs ->
+             NLSC.sem_clock H b ck (abstract_clock xs)).
+
+  Lemma var_inv_weaken:
+    forall (D1 D2 : positive -> Prop) (env : list (ident * clock)),
+      var_inv D1 env ->
+      (forall x, D2 x -> D1 x) ->
+      var_inv D2 env.
+  Proof.
+    intros D1 D2 env I1 H12 x D2x.
+    now apply H12, I1 in D2x.
+  Qed.
+
 
 End LUSTRE_TO_NLUSTRE.
 
