src/Common/CommonList.v
@@ -61,6 +61,55 @@ Section Extra.
     destruct xs; simpl; auto.
   Qed.
 
+  Lemma app_length_impl :
+    forall {A B} (l1 l'1 : list A) (l2 l'2 : list B),
+      length l'1 = length l'2 ->
+      length (l'1 ++ l1) = length (l'2 ++ l2) ->
+      length l1 = length l2.
+  Proof.
+    intros * Hl Hlapp.
+    rewrite 2 app_length in Hlapp.
+    omega.
+  Qed.
+
+  Lemma length_app :
+    forall {A B} (l : list A) (l1 l2 : list B),
+      (length l = length (l1 ++ l2)) ->
+      (exists l1' l2', l = l1' ++ l2'
+                  /\ length l1' = length l1
+                  /\ length l2' = length l2).
+  Proof.
+    intros.
+    rewrite app_length in H.
+    exists (firstn (length l1) l),(skipn (length l1) l). split; [|split].
+    - symmetry. apply firstn_skipn.
+    - rewrite firstn_length. apply Min.min_l. omega.
+    - apply app_length_impl with (l'1 := firstn (length l1) l) (l'2 := l1).
+      rewrite firstn_length. apply Min.min_l. omega.
+      rewrite firstn_skipn. now rewrite app_length.
+  Qed.
+
+  Remark Forall_hd:
+    forall (A : Type) (P : A -> Prop) (x : A) (l : list A),
+      Forall P (x :: l) -> P x.
+  Proof.
+    intros * HF. inv HF. auto.
+  Qed.
+
+  Remark Forall_tl:
+    forall (A : Type) (P : A -> Prop) (x : A) (l : list A),
+      Forall P (x :: l) -> Forall P l.
+  Proof.
+    intros * HF. inv HF. auto.
+  Qed.
+
+  Remark Forall_hd_tl:
+    forall (A : Type) (P : A -> Prop) (x : A) (l : list A),
+      Forall P (x :: l) -> P x /\ Forall P l.
+  Proof.
+    intros * HF. inv HF. auto.
+  Qed.
+
   (* should be in standard lib... *)
   Lemma not_in_cons (x a : A) (l : list A):
     ~ In x (a :: l) <-> x <> a /\ ~ In x l.
@@ -694,6 +743,18 @@ Section ConcatMap.
       firstorder.
   - intro H; decompose record H;
       eapply in_concat'; eauto.
+  Qed.
+
+  Lemma concat_Forall :
+    forall (l' : list (list A)) (l : list A) (P : A -> Prop),
+      Forall P (concat l') ->
+      In l l' ->
+      Forall P l.
+  Proof.
+    intros * Hp Hinl.
+    apply Forall_forall. intros x Hinx.
+    eapply Forall_forall; eauto.
+    apply in_concat. eauto.
   Qed.
 
 End ConcatMap.
@@ -1554,6 +1615,22 @@ Section Forall2.
     - inversion Hall1. inversion Hall2. f_equal; eauto.
   Qed.
 
+  Remark Forall2_hd:
+    forall (A B : Type) (P : A -> B -> Prop)
+      (x : A) (l : list A) (x' : B) (l' : list B),
+      Forall2 P (x :: l) (x' :: l') -> P x x'.
+  Proof.
+    intros * HF. inv HF. auto.
+  Qed.
+
+  Remark Forall2_tl:
+    forall (A B : Type) (P : A -> B -> Prop)
+      (x : A) (l : list A) (x' : B) (l' : list B),
+      Forall2 P (x :: l) (x' :: l') -> Forall2 P l l'.
+  Proof.
+    intros * HF. inv HF. auto.
+  Qed.
+
   Lemma Forall2_combine:
     forall P (xs: list A) (ys: list B),
       Forall2 P xs ys -> Forall (fun x => P (fst x) (snd x)) (combine xs ys).
@@ -1840,6 +1917,36 @@ Section Forall3.
       R x y z ->
       Forall3 l0 l1 l2 ->
       Forall3 (x :: l0) (y :: l1) (z :: l2).
+
+  Lemma Forall3_length :
+    forall (l1 : list A) (l2 : list B) (l3 : list C),
+      Forall3 l1 l2 l3 ->
+      length l1 = length l2
+      /\ length l2 = length l3.
+  Proof.
+    induction 1. tauto. simpl. omega.
+  Qed.
+
+  Lemma Forall3_in_right:
+    forall (xs : list A)
+      (ys : list B) (zs : list C) (z : C),
+      Forall3 xs ys zs ->
+      In z zs -> exists (x : A) (y : B), In x xs /\ In y ys /\ R x y z.
+  Proof.
+    induction 1; simpl. contradiction.
+    destruct 1 as [Heq|Hin].
+    now subst; exists x, y; auto.
+    apply IHForall3 in Hin. destruct Hin as (x' & y' & Hin & Hin' & HP).
+    exists x', y'. eauto.
+  Qed.
+
+  Remark Forall3_tl:
+    forall (x : A)
+      (y : B) (z : C) (l0 : list A) (l1 : list B) (l2 : list C),
+      Forall3 (x :: l0) (y :: l1) (z :: l2) -> Forall3 l0 l1 l2.
+  Proof.
+    intros * HF. inv HF. auto.
+  Qed.
 
 End Forall3.
 
